module Proofs.Adequacy where

open import Data.Bool renaming (Bool to ğ”¹)
open import Data.List
open import Data.Maybe
open import Data.Nat
open import Data.Product
open import Data.String hiding (_++_)
open import Relation.Binary.PropositionalEquality hiding ([_])

open import Expression.Compiler
open import Expression.Evaluator
open import Interpreter.Executor

{-
Proves that if an expression evaluates to a given value n, it can be compiled and
executed up to a point at which the result will be equal to n.
More verbosely: if the result of evaluating an expression is n, there exists a
number of steps k, that when the same expression is compiled and evaluated over k
steps, will produce the result n.
-}

adeq : (T : Set) (e : Exp T) (p : Program) (Ïƒ : State) (n : â„•) â†’
        âŸ¦ e âŸ§ Ïƒ â‰¡ just n â†’ (âˆƒ Î» k â†’ âŸ¨âŸ¨ compile e âŸ©âŸ© [] , Ïƒ , k â‰¡ just [ n ])

-- booleans
adeq .ğ”¹ (B x) p Ïƒ n eq = {!!} 
adeq .ğ”¹ (Â¬ x) p Ïƒ n eq = {!!} 
adeq .ğ”¹ (x & y) p Ïƒ n eq = {!!} 
adeq .ğ”¹ (x âˆ¥ y) p Ïƒ n eq = {!!} 

-- naturals
adeq .â„• (N .n) p Ïƒ n refl = suc zero , refl          -- just (n :: []) is trivially equal to just [ n ]

-- variables
adeq .â„• (V x) p Ïƒ zero eq = {!!}
adeq .â„• (V x) p Ïƒ (suc n) eq = {!!}

-- addition
adeq .â„• (e âŠ• eâ‚) p Ïƒ n eq = {!!}

-- subtraction
adeq .â„• (e âŠ eâ‚) p Ïƒ n eq = {!!}

-- if/else
adeq .â„• (if_then_else e eâ‚ eâ‚‚) p Ïƒ n eq = {!!}


--Refined version of adequacy proof
adeq' : (T : Set) (s : Stack) (e : Exp T) (p : Program) (Ïƒ : State) (n : â„•) â†’
        âŸ¦ e âŸ§ Ïƒ â‰¡ just n â†’ (âˆƒ Î» k â†’ âˆƒ Î» k' â†’ âŸ¨âŸ¨ compile e ++ p âŸ©âŸ© s , Ïƒ , k â‰¡ âŸ¨âŸ¨ p âŸ©âŸ© (n âˆ· s), Ïƒ , k')

-- booleans
adeq' .ğ”¹ s (B x) p Ïƒ n eq = {!!} 
adeq' .ğ”¹ s (Â¬ x) p Ïƒ n eq = {!!}
adeq' .ğ”¹ s (x & y) p Ïƒ n eq = {!!}
adeq' .ğ”¹ s (x âˆ¥ y)  p Ïƒ n eq = {!!}

-- naturals
adeq' .â„• s (N x) p Ïƒ .x refl = suc x , x , refl -- just x â‰¡ just x 

-- variables
adeq' .â„• s (V x) p Ïƒ n eq = {!!}

-- addition
adeq' .â„• s (e âŠ• eâ‚) p Ïƒ n eq = {!!}

-- subtraction
adeq' .â„• s (e âŠ eâ‚) p Ïƒ n eq = {!!}

-- if/else
adeq' .â„• s (if_then_else e eâ‚ eâ‚‚) p Ïƒ n eq = {!!}


{-
The following lemma is used to prove adeq-fail for variables.

V-lemma : (Ïƒ : State) (x : String ) â†’ 
      Ïƒ x â‰¡ nothing â†’ (âŸ¨âŸ¨ Var x âˆ· [] âŸ©âŸ© [] , Ïƒ , suc 0) â‰¡ nothing
V-lemma Ïƒ x p rewrite p = refl

But we can use the aux function instead of this.
-}

{-
Identical to adeq above, except that if the result of evaluation is nothing, there
exists a number of execution steps after which the result will also be nothing.
-}
adeq-fail : (T : Set) (e : Exp T) (p : Program) (Ïƒ : State) (n : â„•) â†’
        âŸ¦ e âŸ§ Ïƒ â‰¡ nothing â†’ (âˆƒ Î» k â†’ âŸ¨âŸ¨ compile e âŸ©âŸ© [] , Ïƒ , k â‰¡ nothing)

-- booleans
adeq-fail .ğ”¹ (B x) p Ïƒ n eq = {!!}
adeq-fail .ğ”¹ (Â¬ x) p Ïƒ n eq = {!!}
adeq-fail .ğ”¹ (x & y) p Ïƒ n eq = {!!}
adeq-fail .ğ”¹ (x âˆ¥ y) p Ïƒ n eq = {!!}


-- naturals
adeq-fail .â„• (N x) p Ïƒ n () -- just x â‰¡ nothing is false

-- variables
adeq-fail .â„• (V x) p Ïƒ n eq = {!!}

-- addition
adeq-fail .â„• (e âŠ• eâ‚) p Ïƒ n eq = {!!}

-- subtraction
adeq-fail .â„• (e âŠ eâ‚) p Ïƒ n eq = {!!}

-- if/else
adeq-fail .â„• (if_then_else e eâ‚ eâ‚‚) p Ïƒ n eq = {!!}
